
<!-- Processed by Id: cwm.py,v 1.197 2007-12-13 15:38:39 syosi Exp -->
<!--     using base file:///home/seebi/Projekte/models/SemanticPingback/namespace.n3-->


<rdf:RDF xmlns="http://www.w3.org/2000/01/rdf-schema#"
    xmlns:dcterms="http://purl.org/dc/terms/"
    xmlns:dc="http://purl.org/dc/elements/1.1/"
    xmlns:doap="http://usefulinc.com/ns/doap#"
    xmlns:foaf="http://xmlns.com/foaf/0.1/"
    xmlns:http="http://www.w3.org/2006/http#"
    xmlns:owl="http://www.w3.org/2002/07/owl#"
    xmlns:pingback="http://purl.org/net/pingback/"
    xmlns:rdf="http://www.w3.org/1999/02/22-rdf-syntax-ns#"
    xmlns:rdfs="http://www.w3.org/2000/01/rdf-schema#"
    xmlns:sioc="http://rdfs.org/sioc/ns#"
    xmlns:skos="http://www.w3.org/2004/02/skos/core#"
    xmlns:vann="http://purl.org/vocab/vann/">

    <owl:Ontology rdf:about="http://purl.org/net/pingback/">
        <label>Semantic Pingback Vocabulary</label>
        <dc:date>2010-09-07</dc:date>
        <foaf:maker rdf:resource="http://www.informatik.uni-leipzig.de/~auer/foaf.rdf#me"/>
        <foaf:maker rdf:resource="http://philipp.frischmuth24.de/id/me"/>
        <foaf:maker rdf:resource="http://sebastian.tramp.name"/>
        <foaf:maker rdf:resource="http://bblfish.net/people/henry/card#me"/>
        <dc:description>This small vocabulary defines resources which are used in the context of Semantic Pingback. The Semantic Pingback mechanism is an extension of the well-known Pingback method, a technological cornerstone of the blogosphere, thus supporting the interlinking within the Data Web.</dc:description>
    </owl:Ontology>
    
    <foaf:Person rdf:about="http://www.informatik.uni-leipzig.de/~auer/foaf.rdf#me">
        <foaf:name>SÃ¶ren Auer</foaf:name>
    </foaf:Person>
    
    <foaf:Person rdf:about="http://philipp.frischmuth24.de/id/me">
        <foaf:name>Philipp Frischmuth</foaf:name>
    </foaf:Person>
    
    <foaf:Person rdf:about="http://sebastian.tramp.name">
        <foaf:name>Sebastian Tramp</foaf:name>
    </foaf:Person>

    <foaf:Person rdf:about="http://bblfish.net/people/henry/card#me">
        <foaf:name>Henry Story</foaf:name>
    </foaf:Person>
    
    
    <owl:Class rdf:about="http://purl.org/net/pingback/Container">
        <isDefinedBy rdf:resource="http://purl.org/net/pingback/"/>
        <label>Pingback Container</label>
        <seeAlso rdf:resource="http://purl.org/net/pingback/Item"/>
        <subClassOf rdf:resource="http://rdfs.org/sioc/ns#Container"/>
        <rdfs:comment>Doing a GET on a pingback:Container with mime type html should return a html form.</rdfs:comment>
        <rdfs:comment>Doing a POST of an pingback:Request on a pingback:Container creates a pingback:Item</rdfs:comment>
    </owl:Class>

    <owl:Class rdf:about="http://purl.org/net/pingback/Item">
        <isDefinedBy rdf:resource="http://purl.org/net/pingback/"/>
        <label>Pingback</label>
        <seeAlso rdf:resource="http://purl.org/net/pingback/Container"/>
        <subClassOf rdf:resource="http://rdfs.org/sioc/ns#Item"/>
        <rdfs:comment>One should be able to do a GET on a pingback:Item instance (and get back an RDFa/n3, RDF/XML document), a DELETE and an PUT (to be defined later).</rdfs:comment>
    </owl:Class>

    <owl:Class rdf:about="http://purl.org/net/pingback/Request">
        <isDefinedBy rdf:resource="http://purl.org/net/pingback/"/>
        <label>(Simplified) Pingback HTTP Request</label>
        <subClassOf rdf:resource="http://www.w3.org/2006/http#PostRequest"/>
        <subClassOf rdf:parseType="Resource">
            <rdf:type rdf:resource="http://www.w3.org/2002/07/owl#Restriction"/>
            <owl:hasValue rdf:resource="http://purl.org/net/pingback/sourceParameter"/>
            <owl:hasValue rdf:resource="http://purl.org/net/pingback/targetParameter"/>
            <owl:maxCardinality rdf:datatype="http://www.w3.org/2001/XMLSchema#int">3</owl:maxCardinality>
            <owl:minCardinality rdf:datatype="http://www.w3.org/2001/XMLSchema#int">2</owl:minCardinality>
            <owl:onProperty rdf:resource="http://www.w3.org/2006/http#param"/>
        </subClassOf>
        <rdfs:comment>This is the class of all REST-based pingback requests. Such a request SHOULD at least have a parameter source and target. </rdfs:comment>
    </owl:Class>

    <owl:Class rdf:about="http://purl.org/net/pingback/RequestGuideline">
        <comment>This concept represents the process of creating data based on a pingback request.</comment>
        <isDefinedBy rdf:resource="http://purl.org/net/pingback/"/>
        <label>Pingback Creation Guideline</label>
        <subClassOf rdf:resource="http://purl.org/net/provenance/ns#CreationGuideline"/>
    </owl:Class>
    

    <owl:ObjectProperty rdf:about="http://purl.org/net/pingback/service">
        <isDefinedBy rdf:resource="http://purl.org/net/pingback/"/>
        <label>pingback service</label>
        <seeAlso rdf:resource="http://hixie.ch/specs/pingback/pingback-1.0"/>
        <rdfs:comment>This property is used to link the target resource with a pingback XML/RPC service URI. The linked service should accept XML/RPC pingback requests as described in the Pingback 1.0 specification.</rdfs:comment>
    </owl:ObjectProperty>

    <owl:ObjectProperty rdf:about="http://purl.org/net/pingback/source">
        <domain rdf:resource="http://purl.org/net/pingback/Item"/>
        <isDefinedBy rdf:resource="http://purl.org/net/pingback/"/>
        <label>source resource</label>
        <skos:example rdf:resource="http://purl.org/net/pingback/examplePingback1"/>
        <skos:example rdf:resource="http://purl.org/net/pingback/examplePingback2"/>
        <rdfs:comment>The source resource of a Pingback (Item) is in most cases the subject of the statement which is communicated with this pingback request.</rdfs:comment>
    </owl:ObjectProperty>
    
    <owl:ObjectProperty rdf:about="http://purl.org/net/pingback/target">
        <domain rdf:resource="http://purl.org/net/pingback/Item"/>
        <isDefinedBy rdf:resource="http://purl.org/net/pingback/"/>
        <label>target resource</label>
        <skos:example rdf:resource="http://purl.org/net/pingback/examplePingback1"/>
        <skos:example rdf:resource="http://purl.org/net/pingback/examplePingback2"/>
        <rdfs:comment>The target resource of a Pingback (Item) is in most cases the object of the statement which is communicated with this pingback request.</rdfs:comment>
    </owl:ObjectProperty>
    
    <owl:ObjectProperty rdf:about="http://purl.org/net/pingback/to">
        <isDefinedBy rdf:resource="http://purl.org/net/pingback/"/>
        <label>pingback request to</label>
        <range rdf:resource="http://purl.org/net/pingback/Container"/>
        <seeAlso rdf:resource="http://aksw.org/Projects/SemanticPingBack#simplepost"/>
        <seeAlso rdf:resource="http://purl.org/net/pingback/Request"/>
        <rdfs:comment>This property is used to link the subject resource (which is then the target resource of the pingback request) with a resource which accept the simplified pingback request. This relation (as well as pingback:service) gives a way for other services to ping this resource e.g. when a new document was created that mentions this resource.</rdfs:comment>
    </owl:ObjectProperty>
    

    

    

    

    <http:Param rdf:about="http://purl.org/net/pingback/commentParameter">
        <isDefinedBy rdf:resource="http://purl.org/net/pingback/"/>
        <label>comment</label>
        <rdfs:comment>The value of this parameter is an URI.</rdfs:comment>
        <http:paramName>comment</http:paramName>
    </http:Param>
    
    <http:Param rdf:about="http://purl.org/net/pingback/sourceParameter">
        <isDefinedBy rdf:resource="http://purl.org/net/pingback/"/>
        <label>source</label>
        <rdfs:comment>The value of this parameter is an URI.</rdfs:comment>
        <http:paramName>source</http:paramName>
    </http:Param>

    <http:Param rdf:about="http://purl.org/net/pingback/targetParameter">
        <isDefinedBy rdf:resource="http://purl.org/net/pingback/"/>
        <label>target</label>
        <rdfs:comment>The value of this parameter is an URI.</rdfs:comment>
        <http:paramName>target</http:paramName>
    </http:Param>
    
</rdf:RDF>
